ground_PDDL_plan.thy
@@ -27,7 +27,7 @@ datatype ('pr, 't) action = GroundAction
     (s_snap: "'pr snap") 
     (oc: "'pr list") 
     (e_snap: "'pr snap")
-    (d_const: "('t dc) option")
+    (d_const: "'t dc option")
 
 text \<open>These orderings are necessary for proofs\<close>
 derive (linorder) compare rat 
@@ -58,6 +58,10 @@ possible to derive the formulation of planning used for the compilation to timed
 The the representations of the state is not necessarily finite, because the initial and final, and 
 thus all states can be infinite in size.\<close>
 
+abbreviation "snap_pre \<equiv> set o pre"
+abbreviation "snap_adds \<equiv> set o adds"
+abbreviation "snap_dels \<equiv> set o dels"
+
 
 locale ground_PDDL_planning =
   fixes props::   "('proposition::linorder) set"
@@ -68,8 +72,8 @@ locale ground_PDDL_planning =
       and some_actions:     "card actions > 0"
       and finite_props:     "finite props"
       and finite_actions:   "finite actions"
+      and act_mod_fluents:  "const_valid_domain props s_snap e_snap snap_adds snap_dels actions"
 begin
-                              
 
   definition lower_imp::"('proposition, rat) action \<rightharpoonup> rat lower_bound" where
   "lower_imp a \<equiv> (case d_const a of 
@@ -85,12 +89,251 @@ begin
   | (Some (duration_op.LEQ, n)) \<Rightarrow> Some (upper_bound.LE n)
   | None \<Rightarrow> None)"
 
-sublocale basic_temp_planning_problem props actions init goal s_snap e_snap "set o oc" 
-  lower_imp upper_imp "set o pre" "set o adds" "set o dels" 0
-  apply standard
-  using some_props some_actions finite_props finite_actions by auto
+
+sublocale finite_fluent_temp_planning_problem' init goal s_snap e_snap "set o oc" 
+  lower_imp upper_imp snap_pre snap_adds snap_dels 0 props actions 
+  apply unfold_locales
+  using some_props some_actions finite_props finite_actions act_mod_fluents by auto
+text \<open>The above locale is a superlocale of the locale below. Now, we can obtain the timed automaton\<close>
+
+sublocale ta_temp_planning 
+    init' goal' AtStart AtEnd over_all' lower_imp upper_imp
+    pre_imp' add_imp' del_imp' 0 props actions ..
 
 
 
 end
+
+
+context
+  fixes ty_ent::  "'ent \<rightharpoonup> type"  \<comment> \<open>Entity's type, None if invalid\<close>
+    and of_type:: "type \<Rightarrow> type \<Rightarrow> bool"
+    and sig::     "predicate \<rightharpoonup> type list"
+begin
+  definition is_of_type :: "'ent \<Rightarrow> type \<Rightarrow> bool" where
+    "is_of_type v T \<longleftrightarrow> (
+      case ty_ent v of
+        Some vT \<Rightarrow> of_type vT T
+      | None \<Rightarrow> False)"
+  
+  fun wf_pred_atom :: "predicate \<times> 'ent list \<Rightarrow> bool" where
+    "wf_pred_atom (p,vs) \<longleftrightarrow> (
+      case sig p of
+        None \<Rightarrow> False
+      | Some Ts \<Rightarrow> list_all2 is_of_type vs Ts)"
+
+  fun wf_pred :: "'ent atom \<Rightarrow> bool" where
+    "wf_pred (predAtm p vs) \<longleftrightarrow> wf_pred_atom (p,vs)"
+  | "wf_pred (eqAtm a b) \<longleftrightarrow> False"
+
+  fun wf_atom :: "'ent atom \<Rightarrow> bool" where
+    "wf_atom (predAtm p vs) \<longleftrightarrow> wf_pred_atom (p,vs)"
+  | "wf_atom (eqAtm a b) \<longleftrightarrow> ty_ent a \<noteq> None \<and> ty_ent b \<noteq> None"
+
+  fun wf_snap::"'ent atom snap \<Rightarrow> bool" where
+    "wf_snap (Snap ps as ds) = (list_all wf_atom ps \<and> list_all wf_pred as \<and> list_all wf_pred ds)"
+
+  fun wf_action::"('ent atom, 'time::time) action \<Rightarrow> bool" where
+    "wf_action (GroundAction n as over_all_cond es dc) = (wf_snap as \<and> list_all wf_atom over_all_cond \<and> wf_snap es)"
+end
+
+locale ground_PDDL_planning_with_equality = 
+  ground_PDDL_planning fluent_preds actions init goal 
+    for fluent_preds::   "('ent::linorder) atom set"
+    and actions:: "('ent atom, rat) action set"
+    and init::    "'ent atom set"
+    and goal::    "'ent atom set"
+   (* fixes ty_ent::  "'ent \<rightharpoonup> type"
+    and of_type:: "type \<Rightarrow> type \<Rightarrow> bool"
+    and sig::     "predicate \<rightharpoonup> type list" *)
+     (*  assumes wf_preds:         "\<forall>p \<in> preds. wf_pred ty_ent of_type sig p"
+      and wf_init:          "\<forall>p \<in> init. wf_pred ty_ent of_type sig p"
+      and wf_goal:          "\<forall>p \<in> goal. wf_pred ty_ent of_type sig p"
+      and wf_actions:       "\<forall>a \<in> actions. wf_action ty_ent of_type sig a" *)
+begin
+
+end
+
+
+abbreviation "person_on_floor \<equiv> Pred ''person_on_floor''"
+abbreviation "elevator_on_floor \<equiv> Pred ''elevator_on_floor''"
+abbreviation "stopped \<equiv> Pred ''stopped''"
+abbreviation "person_in_elevator \<equiv> Pred ''person_in_elevator''"
+
+abbreviation "person1 \<equiv> Obj ''person1''"
+
+abbreviation "floor1 \<equiv> Obj ''floor1''"
+abbreviation "floor2 \<equiv> Obj ''floor2''"
+abbreviation "floor3 \<equiv> Obj ''floor3''"
+
+abbreviation "elevator1 \<equiv> Obj ''elevator1''"
+
+abbreviation "person_locations \<equiv> {
+  predAtm person_on_floor [floor1, person1],
+  predAtm person_on_floor [floor2, person1],
+  predAtm person_on_floor [floor3, person1]
+}"
+
+abbreviation "elevator_locations \<equiv> {
+  predAtm elevator_on_floor [floor1, elevator1],
+  predAtm elevator_on_floor [floor2, elevator1],
+  predAtm elevator_on_floor [floor3, elevator1]
+}"
+
+abbreviation "elevator_stopped \<equiv> {
+  predAtm stopped [elevator1]
+}"
+
+abbreviation "in_elevator \<equiv> {
+  predAtm person_in_elevator [person1, elevator1]
+}"
+
+definition preds::"object atom set" where
+"preds \<equiv> person_locations \<union> elevator_locations \<union> elevator_stopped \<union> in_elevator"
+
+
+text \<open>Move people into elevators\<close>
+abbreviation "mpe111 \<equiv> 
+GroundAction ''mpe111'' 
+  (Snap [predAtm person_on_floor [floor1, person1]] [] [predAtm person_on_floor [floor1, person1]])
+  [predAtm stopped [elevator1], predAtm elevator_on_floor [floor1, elevator1]]
+  (Snap [] [predAtm person_in_elevator [person1, elevator1]] [])
+  (Some (duration_op.EQ, (4::rat)))
+"
+
+abbreviation "mpe112 \<equiv> 
+GroundAction ''mpe112'' 
+  (Snap [predAtm person_on_floor [floor2, person1]] [] [predAtm person_on_floor [floor2, person1]])
+  [predAtm stopped [elevator1], predAtm elevator_on_floor [floor2, elevator1]]
+  (Snap [] [predAtm person_in_elevator [person1, elevator1]] [])
+  (Some (duration_op.EQ, (4::rat)))
+"
+
+abbreviation "mpe113 \<equiv> 
+GroundAction ''mpe113'' 
+  (Snap [predAtm person_on_floor [floor3, person1]] [] [predAtm person_on_floor [floor3, person1]])
+  [predAtm stopped [elevator1], predAtm elevator_on_floor [floor3, elevator1]]
+  (Snap [] [predAtm person_in_elevator [person1, elevator1]] [])
+  (Some (duration_op.EQ, (4::rat)))
+"
+
+text \<open>Move people out of elevators\<close>
+abbreviation "mpf111 \<equiv> 
+GroundAction ''mpf111'' 
+  (Snap [predAtm person_in_elevator [person1, elevator1]] [] [predAtm person_in_elevator [person1, elevator1]])
+  [predAtm stopped [elevator1], predAtm elevator_on_floor [floor1, elevator1]]
+  (Snap [] [predAtm person_on_floor [floor1, person1]] [])
+  (Some (duration_op.EQ, (4::rat)))
+"
+
+abbreviation "mpf112 \<equiv> 
+GroundAction ''mpf112'' 
+  (Snap [predAtm person_in_elevator [person1, elevator1]] [] [predAtm person_in_elevator [person1, elevator1]])
+  [predAtm stopped [elevator1], predAtm elevator_on_floor [floor2, elevator1]]
+  (Snap [] [predAtm person_on_floor [floor2, person1]] [])
+  (Some (duration_op.EQ, (4::rat)))
+"
+
+abbreviation "mpf113 \<equiv> 
+GroundAction ''mpf113'' 
+  (Snap [predAtm person_in_elevator [person1, elevator1]] [] [predAtm person_in_elevator [person1, elevator1]])
+  [predAtm stopped [elevator1], predAtm elevator_on_floor [floor3, elevator1]]
+  (Snap [] [predAtm person_on_floor [floor3, person1]] [])
+  (Some (duration_op.EQ, (4::rat)))
+"
+
+text \<open>Move elevators\<close>
+abbreviation "me112 \<equiv> 
+GroundAction ''me112'' 
+  (Snap [predAtm stopped [elevator1], predAtm elevator_on_floor [floor1, elevator1]] [] [predAtm stopped [elevator1], predAtm elevator_on_floor [floor1, elevator1]])
+  []
+  (Snap [] [predAtm stopped [elevator1], predAtm elevator_on_floor [floor2, elevator1]] [])
+  (Some (duration_op.EQ, (4::rat)))
+"
+
+abbreviation "me113 \<equiv> 
+GroundAction ''me113'' 
+  (Snap [predAtm stopped [elevator1], predAtm elevator_on_floor [floor1, elevator1]] [] [predAtm stopped [elevator1], predAtm elevator_on_floor [floor1, elevator1]])
+  []
+  (Snap [] [predAtm stopped [elevator1], predAtm elevator_on_floor [floor3, elevator1]] [])
+  (Some (duration_op.EQ, (4::rat)))
+"
+
+abbreviation "me121 \<equiv> 
+GroundAction ''me121'' 
+  (Snap [predAtm stopped [elevator1], predAtm elevator_on_floor [floor2, elevator1]] [] [predAtm stopped [elevator1], predAtm elevator_on_floor [floor2, elevator1]])
+  []
+  (Snap [] [predAtm stopped [elevator1], predAtm elevator_on_floor [floor1, elevator1]] [])
+  (Some (duration_op.EQ, (4::rat)))
+"
+
+abbreviation "me123 \<equiv> 
+GroundAction ''me123'' 
+  (Snap [predAtm stopped [elevator1], predAtm elevator_on_floor [floor2, elevator1]] [] [predAtm stopped [elevator1], predAtm elevator_on_floor [floor2, elevator1]])
+  []
+  (Snap [] [predAtm stopped [elevator1], predAtm elevator_on_floor [floor3, elevator1]] [])
+  (Some (duration_op.EQ, (4::rat)))
+"
+
+abbreviation "me131 \<equiv> 
+GroundAction ''me131'' 
+  (Snap [predAtm stopped [elevator1], predAtm elevator_on_floor [floor3, elevator1]] [] [predAtm stopped [elevator1], predAtm elevator_on_floor [floor3, elevator1]])
+  []
+  (Snap [] [predAtm stopped [elevator1], predAtm elevator_on_floor [floor1, elevator1]] [])
+  (Some (duration_op.EQ, (4::rat)))
+"
+
+abbreviation "me132 \<equiv> 
+GroundAction ''me132'' 
+  (Snap [predAtm stopped [elevator1], predAtm elevator_on_floor [floor3, elevator1]] [] [predAtm stopped [elevator1], predAtm elevator_on_floor [floor3, elevator1]])
+  []
+  (Snap [] [predAtm stopped [elevator1], predAtm elevator_on_floor [floor2, elevator1]] [])
+  (Some (duration_op.EQ, (4::rat)))
+"
+
+definition actions::"(object atom, rat) action set" where
+"actions \<equiv> {mpe111, mpe112, mpe113, mpf111, mpf112, mpf113, me112, me113, me121, me123, me131, me132}"
+
+definition init::"object atom set" where
+"init \<equiv> {predAtm person_on_floor [floor1, person1]}"
+
+definition goal::"object atom set" where
+"goal \<equiv> {predAtm person_on_floor [floor3, person1]}"
+
+
+global_interpretation ground_PDDL_planning_with_equality preds actions init goal
+proof
+  show "finite preds" unfolding preds_def by blast
+  moreover 
+  have "\<exists>x. x \<in> preds" unfolding preds_def by blast
+  ultimately
+  show "0 < card preds" using card_gt_0_iff by blast
+
+  show "finite actions" unfolding actions_def by blast
+  moreover
+  have "\<exists>x. x \<in> actions" unfolding actions_def by blast
+  ultimately
+  show "0 < card actions" using card_gt_0_iff by blast
+
+  show "const_valid_domain preds s_snap e_snap snap_adds snap_dels actions"
+    unfolding const_valid_domain_def act_mod_fluents_def
+  proof (intro ballI; intro conjI)
+    fix a
+    assume a: "a \<in> actions"
+    consider "a = mpe111" | "a = mpe112" | "a = mpe113" 
+      | "a = mpf111" | "a = mpf112" | "a = mpf113" 
+      | "a = me112" | "a = me113" | "a = me121" 
+      | "a = me123" | "a = me131" | "a = me132" 
+      by (insert a[simplified actions_def, simplified], elim disjE, assumption+) 
+    note ac = this
+    show "snap_mod_fluents preds snap_adds snap_dels (s_snap a)" 
+      by (cases rule: ac; simp add: preds_def)
+    show "snap_mod_fluents preds snap_adds snap_dels (e_snap a)"
+      by (cases rule: ac; simp add: preds_def)
+  qed
+qed
+
+
+ML \<open>\<close>
+      
 end
